\begin{proof}

	\begin{align*}
		\forall X \in M_{n \times m}\, f_X & : \vec b \mapsto X \vec b \\
		                                   & : \R^{m} \to \R^n
	\end{align*}
	\begin{align*}
		\llet C & = \mat{ T(\vec x_1) & T(\vec x_2) & \cdots & T(\vec x_k) } \\
		\llet B & = \mat{ \vec x_1    & \vec x_2    & \cdots & \vec x_k }    \\
		C       & = A \circ B
	\end{align*}
	\begin{align*}
		f_C                                             & = T \circ f_B                                     \\
		\mathcal L_{1} \implies		\forall \vec a, \vec b & :\, f_C(\vec a) = f_C(\vec b) \iff  \vec a=\vec b
	\end{align*}

	\begin{align*}
		\llet \vec b, \vec c   & \in \R^{k}              \\
		f_B (\vec b)           & = f_B(\vec c)           \\
		(T \circ	f_B) (\vec b) & = (T \circ f_B)(\vec c) \\
		f_C (\vec b)           & = f_C(\vec c)           \\
		\vec b                 & = \vec c
	\end{align*}
	\begin{align*}
		                          & \therefore                 f_B \text{ is injective}                                   \\
		                          & \implies \forall \vec b, \vec c \in \R^{k} :\, B\vec b = B\vec c \iff \vec b = \vec c \\
		                          & \implies \forall \vec b \in \R^{k} :\, B\vec b = \vec 0 \iff \vec b = \vec 0          \\
		\dots \wedge	\mathcal L_2 & \implies \set{\vec x_1, \vec x_2 , \cdots , \vec x_k} \text{is linearly independent.}
	\end{align*}

\end{proof}
